Velvet2/Examples/AutomaticExceptionInference.lean
@@ -1,5 +1,4 @@
 import Velvet2.Syntax
-import Velvet2.Tactics
 import Velvet2.VCGen.Frontend
 
 /-
